WhileD/WhileDCompleteness.v
@@ -4,6 +4,7 @@ Require Import Coq.Lists.List.
 Require Import Coq.Strings.String.
 Require Import Coq.ZArith.ZArith.
 Require Import Coq.micromega.Psatz.
+Require Import compcert.lib.Integers.
 Require Import SetsClass.SetsClass. Import SetsNotation.
 Require Import PV.Syntax.
 Require Import PV.WhileDDenotations.
@@ -22,7 +23,9 @@ Import HoareWhileD.
 Import HoareWhileD_Admissible.
 
 Definition wp (c:com) (Q:assertion) : assertion :=
-  fun s => forall s', (eval_com c).(nrm) s s' -> Q s'.
+  fun s => forall s',
+  ((eval_com c).(err) s -> False) /\
+  ((eval_com c).(nrm) s s' -> Q s').
 
 Hint Unfold wp : core.
 
@@ -34,8 +37,11 @@ Proof.
   intros s1 s2.
   unfold wp.
   intros.
-  apply H.
-  tauto.
+  split.
+  + apply H.
+  + intros.
+    specialize (H s1).
+    tauto.
 Qed.
 
 Theorem wp_is_weakest : forall c Q P',
@@ -47,12 +53,14 @@ Proof.
   unfold wp.
   intros.
   specialize (H s s').
+  split; intros;
   apply H; tauto.
 Qed.
 
 Lemma wp_seq : forall P Q c1 c2,
     provable {{P}} c1 {{(wp c2 Q)}} -> 
-    provable {{(wp c2 Q)}} c2 {{Q}} -> provable {{P}} (c1; c2) {{Q}}.
+    provable {{(wp c2 Q)}} c2 {{Q}} ->
+    provable {{P}} (c1; c2) {{Q}}.
 Proof.
   intros.
   eapply hoare_seq; [apply H|apply H0].
@@ -67,32 +75,89 @@ Proof.
   simpl.
   intros.
   destruct H.
-  specialize (H s').
-  apply H.
-  revert H1 H2 H0.
-  simpl.
-  unfold while_sem.
-  unfold_RELS_tac.
-  intros.
-  destruct H1.
-  exists (S x).
-  simpl.  
-  unfold_RELS_tac.
-  left.
-  exists s1.
-  split.
-  + unfold test_true.
+  split; intros.
+  + specialize (H s').
+    destruct H.
+    split.
+    - intros.
+      apply H.
+      revert H3; unfold_RELS_tac; intros.
+      destruct H3 as [i ?].
+      exists (S i).
+      simpl.
+      unfold_RELS_tac.
+      left.
+      exists s1.
+      split. {
+        unfold test_true.
+        unfold eb2assn in H0.
+        unfold_RELS_tac.
+        tauto.
+      }
+      left.
+      exists s2.
+      tauto.
+    - intros.
+      apply H2.
+      revert H3; unfold_RELS_tac; intros.
+      destruct H3 as [i ?].
+      exists (S i).
+      simpl.
+      unfold_RELS_tac.
+      left.
+      exists s1.
+      split. {
+        unfold test_true.
+        unfold eb2assn in H0.
+        unfold_RELS_tac.
+        tauto.
+      }
+      exists s2.
+      tauto.
+  + specialize (H s1); destruct H.
+    apply H.
     unfold_RELS_tac.
-    split; [|tauto].
-    revert H2.
-    unfold eb2assn. tauto.
-  + exists s2.
-    tauto.
+    exists (S O).
+    simpl.
+    unfold_RELS_tac.
+    left.
+    exists s1.
+    split. {
+      unfold test_true.
+      unfold eb2assn in H0.
+      unfold_RELS_tac.
+      tauto.
+    }
+    right; tauto.
 Qed.
 (* 
 Lemma concat_empty: 
   forall X,
   Rels.concat X Sets.empty = Sets.empty. *)
+
+Definition expr_equal_to(e : expr)(a : int64) : assertion :=
+  fun s => (eval_r e).(nrm) s a.
+
+Definition var_env_equal_to(x : var_name)(a : int64) : assertion :=
+  fun s => s.(env) x = a.  
+
+Definition exp_state(s : state)(a : int64)(P : assertion) : Prop :=
+  exists v : val, P (state_subst s a v).
+
+Definition exclude_mem(P : assertion)(a : int64) : assertion :=
+  fun s => (s.(mem) a = None /\ (exp_state s a P)).
+
+Definition one_mem_state(s:state)(a:int64) : state :=
+  {|
+    env := s.(env);
+    mem := fun y => if (Int64.eq y a) then s.(mem) a else None;
+  |}.
+  
+Definition exclude_one_mem_state(s:state)(a:int64) : state :=
+  {|
+    env := s.(env);
+    mem := fun y => if (Int64.eq y a) then None else s.(mem) y;
+  |}.
 
 Theorem hoare_complete: forall P Q c,
    valid {{ P }} c {{ Q }} -> provable {{ P }} c {{ Q }}.
@@ -112,93 +177,563 @@ Proof.
       reflexivity.
     - eapply hoare_conseq_post; [|apply H].
       apply (hoare_skip P).
-  + admit.
-  + unfold eval_com in HT.
-    simpl in HT.
-    assert(exists a, (forall (s:state), P s -> ((eval_r e1).(nrm) s a))).
-    admit.
-    assert(exists b, (forall (s:state), P s -> ((eval_r e2).(nrm) s b))).
-    admit.
-    destruct H as [a ?].
-    destruct H0 as [b ?].
-    pose proof hoare_asgn_deref_fwd P Q e1 e2 a b.
-    pose proof H1 H H0.
-    clear H1.
-    assert(P |-- exp (fun u : val => Assn ((store a u) * Q))).
-    - unfold sepcon.
-      unfold store.
+  + assert(P |-- (exp64 (fun a:int64 => (andp P (var_env_equal_to x a))))). {
       unfold derives.
+      unfold exp64.
+      unfold var_env_equal_to.
+      unfold andp.
       intros.
-      unfold exp.
-       
-    destruct H2.
-    apply H1 in H; auto.
-    - apply (hoare_conseq_post _ _ _ _ H).
-      unfold sepcon.
+      exists (s.(env) x).
+      tauto.
+    }
+    eapply hoare_conseq_pre; [|apply H].
+    apply hoare_exist.
+    intros.
+    assert(P |-- (exp64 (fun b:int64 => (andp P (expr_equal_to e b))))). {
       unfold derives.
+      unfold exp64.
+      unfold expr_equal_to.
+      unfold andp.
       intros.
-      destruct H2 as [s11 [s12 ?]].
-      destruct H2 as [? [? [? [? ?]]]].
-      specialize (HT ).
-    - 
+      specialize (HT s s H0).
+      destruct HT.
+      simpl in H2.
+      revert H2; unfold_RELS_tac; intros.
+      assert ((eval_r e).(err) s -> False) by tauto.
+      pose proof eval_r_not_err _ _ H3.
+      destruct H4.
+      exists x0.
+      tauto.
+    }
+    assert (Assn(P && (var_env_equal_to x a)) |-- exp64 (fun b : int64 => Assn (P && (var_env_equal_to x a) && (expr_equal_to e b)))). {
+      revert H0.
+      unfold derives, exp64, andp.
+      intros.
+      destruct H1.
+      specialize (H0 s H1).
+      destruct H0.
+      exists x0.
+      tauto.
+    }
+    eapply hoare_conseq_pre; [|apply H1].
+    apply hoare_exist.
+    intro a0.
+    clear H H0 H1.
+    pose proof hoare_asgn_var_fwd (Assn(P && (var_env_equal_to x a) && (expr_equal_to e a0))) (exclude_mem Assn(P && (var_env_equal_to x a) && (expr_equal_to e a0)) a).
+    specialize (H e a a0 x).
+    assert((forall s : state, Assn (P && (var_env_equal_to x a) && (expr_equal_to e a0)) s -> s.(env) x = a)). {
+      clear H.
+      intros.
+      unfold andp in H.
+      destruct H.
+      destruct H.
+      unfold var_env_equal_to in H1.
+      apply H1.
+    }
+    assert((forall s : state, Assn (P && (var_env_equal_to x a) && (expr_equal_to e a0)) s -> (eval_r e).(nrm) s a0)). {
+      clear H.
+      intros.
+      unfold andp in H.
+      destruct H.
+      destruct H.
+      unfold expr_equal_to in H1.
+      apply H1.
+    }
+    assert((Assn (P && (var_env_equal_to x a) && (expr_equal_to e a0)))
+    |--  exp (fun u : val => (sepcon (store a u) (exclude_mem (Assn (P && (var_env_equal_to x a) && (expr_equal_to e a0))) a)))). {
+      clear H H0 H1.
+      unfold sepcon, andp, exp, expr_equal_to, var_env_equal_to, store, derives, exp_state, state_subst.
+      intros.
+      destruct H.
+      destruct H.
+      specialize (HT s s H).
+      destruct HT.
+      simpl in H3.
+      revert H3; unfold_RELS_tac; intros.
+      assert(asgn_deref_sem_err (fun (s : state) (i : int64) => s.(env) x = i) s -> False) by tauto.
+      (* assert(asgn_deref_sem_err (eval_r e1).(nrm) s -> False) by tauto. *)
+      clear H3.
+      unfold asgn_deref_sem_err in H4.
+      assert (exists u: val, s.(mem) a = Some u). {
+        destruct (s.(mem) a) eqn : I.
+        - exists v; tauto.
+        - destruct H4.
+          exists a.
+          tauto.
+      }
+      destruct H3.
+      exists x0.
+      exists (one_mem_state s a), (exclude_one_mem_state s a).
+      split.
+      - simpl. 
+        split.
+        * destruct (Int64.eq a a) eqn : J.
+          ++ tauto.
+          ++ rewrite Int64.eq_true in J.
+             discriminate.
+        * intros.
+          destruct (Int64.eq i a) eqn : J.
+          ++ pose proof Int64.eq_false _ _ H5.
+             rewrite J in H6; discriminate.
+          ++ tauto.
+      - split. {
+        unfold exclude_mem.
+        unfold exclude_one_mem_state.
+        split.
+        * simpl.
+          destruct (Int64.eq a a) eqn : J.
+          ++ tauto.
+          ++ rewrite Int64.eq_true in J.
+            discriminate.
+        * unfold exp_state.
+          unfold state_subst; simpl.
+          exists x0.
+          assert((  {|
+          env := s.(env);
+          mem := fun x1 : int64 =>
+                 if Int64.eq x1 a
+                 then Some x0
+                 else if Int64.eq x1 a then None else s.(mem) x1 |}) = s). {
+            assert((fun x1 : int64 =>
+            if Int64.eq x1 a then Some x0 else if Int64.eq x1 a then None else s.(mem) x1) = s.(mem)). {
+              apply functional_extensionality.
+              intros.
+              pose proof Int64.eq_spec x1 a.
+              destruct (Int64.eq x1 a) eqn : K.
+              ++ rewrite H5.
+                 rewrite H3.
+                 reflexivity.
+              ++ reflexivity. 
+            }
+            rewrite H5.
+            destruct s.
+            simpl.
+            reflexivity.
+          }
+          rewrite ! H5.
+          tauto.
+      }
+      split. {
+        unfold one_mem_state.
+        simpl.
+        reflexivity.
+      }
+      split. {
+        unfold exclude_one_mem_state.
+        simpl.
+        reflexivity.
+      }
+      intros. simpl.
+      pose proof Int64.eq_spec i a.
+      destruct (Int64.eq i a) eqn : I.
+      * left.
+        rewrite H5.
+        tauto.
+      * right.
+        tauto.
+    }
+    specialize (H H1 H0 H2).
+    clear H0 H1 H2.
+    apply (hoare_conseq_post _ _ _ _ H).
+    clear H.
+    unfold derives, andp, exclude_mem, expr_equal_to, store, sepcon.
+    intros.
+    destruct H as [s1 [s2 [? [? [? [? ?]]]]]].
+    destruct H.
+    destruct H0.
+    unfold exp_state in H5.
+    destruct H5 as [v ?].
+    destruct H5 as [[? ?] ?].
+    specialize (HT (state_subst s2 a v) s H5).
+    destruct HT.
+    apply H8.
+    simpl.
+    unfold asgn_deref_sem_nrm.
+    exists a, a0.
+    split; [auto | split; auto].
+    split. {
+      unfold state_subst; simpl.
+      pose proof Int64.eq_spec a a.
+      destruct (Int64.eq a a).
+      + discriminate.
+      + contradiction.
+    }
+    split. {
+      specialize (H3 a).
+      destruct H3.
+      + destruct H3.
+        rewrite H3, H.
+        reflexivity.
+      + destruct H3.
+        rewrite H in H10.
+        discriminate. 
+    }
+    split. {
+      intros.
+      unfold state_subst; simpl.
+      rewrite H2.
+      reflexivity.
+    }
+    intros.
+    unfold state_subst; simpl.
+    pose proof Int64.eq_spec p a.
+    destruct (Int64.eq p a).
+    - rewrite H11 in H10; contradiction.
+    - specialize (H3 p).
+      specialize (H4 p H11).
+      destruct H3; destruct H3.
+      * rewrite H4 in H3.
+        rewrite H3.
+        rewrite H12.
+        reflexivity.
+      * rewrite H3.
+        reflexivity.
+  + assert(P |-- (exp64 (fun a:int64 => (andp P (expr_equal_to e1 a))))). {
+      unfold derives.
+      unfold exp64.
+      unfold expr_equal_to.
+      unfold andp.
+      intros.
+      specialize (HT s s H).
+      destruct HT.
+      simpl in H1.
+      revert H1; unfold_RELS_tac; intros.
+      assert ((eval_r e1).(err) s -> False) by tauto.
+      pose proof eval_r_not_err _ _ H2.
+      destruct H3.
+      exists x.
+      tauto.
+    }  
+    eapply hoare_conseq_pre; [|apply H].
+    apply hoare_exist.
+    intros.
+    assert(P |-- (exp64 (fun b:int64 => (andp P (expr_equal_to e2 b))))). {
+      unfold derives.
+      unfold exp64.
+      unfold expr_equal_to.
+      unfold andp.
+      intros.
+      specialize (HT s s H0).
+      destruct HT.
+      simpl in H2.
+      revert H2; unfold_RELS_tac; intros.
+      assert ((eval_r e2).(err) s -> False) by tauto.
+      pose proof eval_r_not_err _ _ H3.
+      destruct H4.
+      exists x.
+      tauto.
+    }
+    assert (Assn(P && (expr_equal_to e1 a)) |-- exp64 (fun b : int64 => Assn (P && (expr_equal_to e1 a) && (expr_equal_to e2 b)))). {
+      revert H0.
+      unfold derives, exp64, andp.
+      intros.
+      destruct H1.
+      specialize (H0 s H1).
+      destruct H0.
+      exists x.
+      tauto.
+    }
+    eapply hoare_conseq_pre; [|apply H1].
+    apply hoare_exist.
+    intro a0.
+    clear H H0 H1.
+    pose proof hoare_asgn_deref_fwd (Assn(P && (expr_equal_to e1 a) && (expr_equal_to e2 a0))) (exclude_mem Assn(P && (expr_equal_to e1 a) && (expr_equal_to e2 a0)) a).
+    specialize (H e1 e2 a a0).
+    assert((forall s : state, Assn (P && (expr_equal_to e1 a) && (expr_equal_to e2 a0)) s -> (eval_r e1).(nrm) s a)). {
+      clear H.
+      intros.
+      unfold andp in H.
+      destruct H.
+      destruct H.
+      unfold expr_equal_to in H1.
+      apply H1.
+    }
+    assert((forall s : state, Assn (P && (expr_equal_to e1 a) && (expr_equal_to e2 a0)) s -> (eval_r e2).(nrm) s a0)). {
+      clear H.
+      intros.
+      unfold andp in H.
+      destruct H.
+      destruct H.
+      unfold expr_equal_to in H1.
+      apply H1.
+    }
+    assert((Assn (P && (expr_equal_to e1 a) && (expr_equal_to e2 a0)))
+    |--  exp (fun u : val => (sepcon (store a u) (exclude_mem (Assn (P && (expr_equal_to e1 a) && (expr_equal_to e2 a0))) a)))). {
+      clear H H0 H1.
+      unfold sepcon, andp, exp, expr_equal_to, store, derives, exp_state, state_subst.
+      intros.
+      destruct H.
+      destruct H.
+      specialize (HT s s H).
+      destruct HT.
+      simpl in H3.
+      revert H3; unfold_RELS_tac; intros.
+      assert(asgn_deref_sem_err (eval_r e1).(nrm) s -> False) by tauto.
+      clear H3.
+      unfold asgn_deref_sem_err in H4.
+      assert (exists u: val, s.(mem) a = Some u). {
+        destruct (s.(mem) a) eqn : I.
+        - exists v; tauto.
+        - destruct H4.
+          exists a.
+          tauto.
+      }
+      destruct H3.
+      exists x.
+      exists (one_mem_state s a), (exclude_one_mem_state s a).
+      split.
+      - simpl. 
+        split.
+        * destruct (Int64.eq a a) eqn : J.
+          ++ tauto.
+          ++ rewrite Int64.eq_true in J.
+             discriminate.
+        * intros.
+          destruct (Int64.eq i a) eqn : J.
+          ++ pose proof Int64.eq_false _ _ H5.
+             rewrite J in H6; discriminate.
+          ++ tauto.
+      - split. {
+        unfold exclude_mem.
+        unfold exclude_one_mem_state.
+        split.
+        * simpl.
+          destruct (Int64.eq a a) eqn : J.
+          ++ tauto.
+          ++ rewrite Int64.eq_true in J.
+            discriminate.
+        * unfold exp_state.
+          unfold state_subst; simpl.
+          exists x.
+          assert((  {|
+          env := s.(env);
+          mem := fun x0 : int64 =>
+                 if Int64.eq x0 a
+                 then Some x
+                 else if Int64.eq x0 a then None else s.(mem) x0 |}) = s). {
+            assert((fun x0 : int64 =>
+            if Int64.eq x0 a then Some x else if Int64.eq x0 a then None else s.(mem) x0) = s.(mem)). {
+              apply functional_extensionality.
+              intros.
+              pose proof Int64.eq_spec x0 a.
+              destruct (Int64.eq x0 a) eqn : K.
+              ++ rewrite H5.
+                 rewrite H3.
+                 reflexivity.
+              ++ reflexivity. 
+            }
+            rewrite H5.
+            destruct s.
+            simpl.
+            reflexivity.
+          }
+          rewrite ! H5.
+          tauto.
+      }
+      split. {
+        unfold one_mem_state.
+        simpl.
+        reflexivity.
+      }
+      split. {
+        unfold exclude_one_mem_state.
+        simpl.
+        reflexivity.
+      }
+      intros. simpl.
+      pose proof Int64.eq_spec i a.
+      destruct (Int64.eq i a) eqn : I.
+      * left.
+        rewrite H5.
+        tauto.
+      * right.
+        tauto.
+    }
+    specialize (H H0 H1 H2).
+    clear H0 H1 H2.
+    apply (hoare_conseq_post _ _ _ _ H).
+    clear H.
+    unfold derives, andp, exclude_mem, expr_equal_to, store, sepcon.
+    intros.
+    destruct H as [s1 [s2 [? [? [? [? ?]]]]]].
+    destruct H.
+    destruct H0.
+    unfold exp_state in H5.
+    destruct H5 as [v ?].
+    destruct H5 as [[? ?] ?].
+    specialize (HT (state_subst s2 a v) s H5).
+    destruct HT.
+    apply H8.
+    simpl.
+    unfold asgn_deref_sem_nrm.
+    exists a, a0.
+    split; [auto | split; auto].
+    split. {
+      unfold state_subst; simpl.
+      pose proof Int64.eq_spec a a.
+      destruct (Int64.eq a a).
+      + discriminate.
+      + contradiction.
+    }
+    split. {
+      specialize (H3 a).
+      destruct H3.
+      + destruct H3.
+        rewrite H3, H.
+        reflexivity.
+      + destruct H3.
+        rewrite H in H10.
+        discriminate. 
+    }
+    split. {
+      intros.
+      unfold state_subst; simpl.
+      rewrite H2.
+      reflexivity.
+    }
+    intros.
+    unfold state_subst; simpl.
+    pose proof Int64.eq_spec p a.
+    destruct (Int64.eq p a).
+    - rewrite H11 in H10; contradiction.
+    - specialize (H3 p).
+      specialize (H4 p H11).
+      destruct H3; destruct H3.
+      * rewrite H4 in H3.
+        rewrite H3.
+        rewrite H12.
+        reflexivity.
+      * rewrite H3.
+        reflexivity.
   + apply (hoare_seq P (fun s => exists x: state, P x /\ (eval_com c1).(nrm) x s) Q).
     - apply IHc1.
       intros.
-      exists s1.
-      tauto.
+      split.
+      * exists s1.
+        tauto.
+      * intros.
+        specialize (HT s1 s1 H).
+        destruct HT.
+        apply H2.
+        simpl.
+        unfold_RELS_tac.
+        tauto.
     - apply IHc2.
       intros.
       destruct H,H.
       specialize (HT x s2).
-      apply HT; [tauto|].
-      simpl.
-      unfold seq_sem.
-      unfold_RELS_tac.
-      exists s1; tauto.
+      split. {
+        specialize (HT H).
+        destruct HT.
+        intros.
+        apply H1.
+        simpl.
+        unfold_RELS_tac.
+        exists s1; tauto.
+      }
+      specialize (HT H); destruct HT.
+      intros.
+      apply H2.
+      simpl; unfold_RELS_tac.
+      right.
+      exists s1.
+      tauto.
   + apply hoare_if.
     - specialize (IHc1 Assn(P && (eb2assn e)) Q).
       apply IHc1.
       intros.
-      specialize (HT s1 s2); apply HT.
-      * revert H. assn_unfold. tauto.
-      * simpl.
-        unfold if_sem.
+      split. {
+        specialize (HT s1 s2).
+        revert H. assn_unfold.
+        intros.
+        destruct H.
+        specialize (HT H).
+        destruct HT; apply H2.
+        simpl.
+        unfold_RELS_tac.
         left.
+        exists s1.
+        unfold eb2assn in H1.
+        destruct H1.
         unfold test_true.
         unfold_RELS_tac.
-        exists s1.
-        split; auto.
-        split; auto.
-        revert H; assn_unfold; tauto.
+        split.
+        * split; auto.
+          exists x; tauto.
+        * tauto.
+      }
+      specialize (HT s1 s2).
+      revert H. assn_unfold.
+      intros.
+      destruct H.
+      specialize (HT H).
+      destruct HT; apply H3.
+      simpl.
+      unfold_RELS_tac.
+      left; right.
+      exists s1.
+      unfold eb2assn in H1.
+      destruct H1.
+      unfold test_true.
+      unfold_RELS_tac.
+      split.
+      * split; auto.
+        exists x; tauto.
+      * tauto.
     - specialize (IHc2 Assn(P && (eb2assn_not e)) Q).
       apply IHc2.
       intros.
-      specialize (HT s1 s2); apply HT.
-      * revert H. assn_unfold. tauto.
-      * simpl.
-        unfold if_sem.
-        right.
-        unfold test_false.
-        unfold_RELS_tac.
-        exists s1.
-        split; auto.
-        split; auto.
-        revert H; assn_unfold.
-        unfold eb2assn.
-        simpl.
-        unfold not_sem.
+      split. {
+        specialize (HT s1 s2).
+        revert H. assn_unfold.
         intros.
-        unfold negb in H; destruct H.
+        destruct H.
+        specialize (HT H).
+        destruct HT; apply H2.
+        simpl.
+        unfold_RELS_tac.
+        right.
+        exists s1.
         unfold eb2assn_not in H1.
         destruct H1.
+        unfold test_false.
+        unfold_RELS_tac.
+        split.
+        * split; auto.
+          destruct H1.
+          rewrite <- H4.
+          pose proof Int64.repr_signed x.
+          rewrite H5.
+          tauto.
+        * tauto. 
+      }
+      specialize (HT s1 s2).
+      revert H. assn_unfold.
+      intros.
+      destruct H.
+      specialize (HT H).
+      destruct HT; apply H3.
+      simpl.
+      unfold_RELS_tac.
+      right.
+      exists s1.
+      unfold eb2assn_not in H1.
+      destruct H1.
+      unfold test_false.
+      unfold_RELS_tac.
+      split.
+      * split; auto.
         destruct H1.
-        assert(x = Integers.Int64.repr 0).
-        ++  rewrite <- H2.
-            pose proof Integers.Int64.repr_signed x.
-            rewrite H3.
-            reflexivity.
-        ++  subst x.
-            tauto. 
+        rewrite <- H4.
+        pose proof Int64.repr_signed x.
+        rewrite H5.
+        tauto.
+      * tauto. 
+    - intros.
+      specialize (HT s s H).
+      destruct HT; apply H2.
+      simpl. unfold_RELS_tac. 
+      tauto.
   + pose proof wp_invariant e c Q.
     specialize (IHc  Assn((wp (CWhile e c) Q) && (eb2assn e))  (wp (CWhile e c) Q)).
     unfold valid in H.
@@ -244,4 +779,15 @@ Proof.
           reflexivity.
       ++  subst x.
           tauto.
+    - intros.
+      unfold wp in H0.
+      specialize (H0 s).
+      destruct H0.
+      apply H0.
+      simpl.
+      unfold_RELS_tac.
+      exists (S O).
+      simpl.
+      unfold_RELS_tac.
+      right; tauto.
 Qed.
